a.v
@@ -4,25 +4,42 @@ Require Import Structures.Orders.
 Require Import Coq.Arith.PeanoNat.
 Require Import Coq.Bool.Bool.
 Require Import Coq.Arith.Arith.
+Require Import Lia.
 Import ListNotations.
 
 Section AMod.
 
 
 
-Inductive Opt: Set :=
-| fail : Opt
-| ok : bool -> Opt.
+(* a real challenge in induction *)
 
 
-Theorem get: forall x: Opt, x<>fail -> bool.
-    refine (fun x:Opt => 
-    match x return x <> fail ->bool with
-    | fail => _ 
-    | ok b => fun _ =>b
-    end ).
-    intros; absurd(fail = fail).
-    
+Variable steps: nat->nat. 
+
+Hypothesis step_0:
+    steps 0 = 0.
+Hypothesis step_increment:
+    forall n:nat, steps n < 10 -> steps (S n) = steps n + 1.
+
+Hypothesis step_increment2:
+    forall n:nat, (steps n)>=10 -> steps (S n) = steps n. 
+
+Theorem bound: forall n:nat, steps n <= 10.
+
+    intros.
+    induction n.
+    rewrite -> step_0.
+    lia.
+    remember (10 -(steps n)) as x.
+    destruct_with_eqn x.
+    assert (steps n = 10) by lia.
+    rewrite -> step_increment2.
+    lia.
+    lia.
+    assert (steps n < 10) by lia.
+    rewrite -> step_increment.
+    lia.
+    trivial.
 
 Qed.
 
